src/PushButtonSynthesis/WordByWordMontgomeryReificationCache.v
@@ -82,7 +82,7 @@ print((indent + '(' + r'''**
 >>
 *''' + ')\n') % open(__file__, 'r').read())
 
-for i in ('mul', 'add', 'sub', 'opp', 'to_bytes', 'from_bytes', 'nonzero', 'eval', 'bytes_eval'):
+for i in ('mul', 'add', 'sub', 'opp', 'scmul' 'to_bytes', 'from_bytes', 'nonzero', 'eval', 'bytes_eval'):
     print((r'''%sDerive reified_%s_gen
        SuchThat (is_reification_of reified_%s_gen %smod)
        As reified_%s_gen_correct.
@@ -159,6 +159,15 @@ Local Opaque reified_%s_gen. (* needed for making [autorewrite] not take a very 
   Hint Immediate (proj2 reified_opp_gen_correct) : wf_gen_cache.
   Hint Rewrite (proj1 reified_opp_gen_correct) : interp_gen_cache.
   Local Opaque reified_opp_gen. (* needed for making [autorewrite] not take a very long time *)
+
+  Derive reified_scmul_gen
+         SuchThat (is_reification_of reified_scmul_gen scmulmod)
+         As reified_scmul_gen_correct.
+  Proof. Time cache_reify (). Time Qed.
+  Hint Extern 1 (_ = _) => apply_cached_reification scmulmod (proj1 reified_scmul_gen_correct) : reify_cache_gen.
+  Hint Immediate (proj2 reified_scmul_gen_correct) : wf_gen_cache.
+  Hint Rewrite (proj1 reified_scmul_gen_correct) : interp_gen_cache.
+  Local Opaque reified_scmul_gen. (* needed for making [autorewrite] not take a very long time *)
 
   Derive reified_to_bytes_gen
          SuchThat (is_reification_of reified_to_bytes_gen to_bytesmod)
