Makefile
@@ -160,6 +160,7 @@ endef
 UNSATURATED_SOLINAS_FUNCTIONS := carry_mul carry_square carry add sub opp selectznz to_bytes from_bytes
 FUNCTIONS_FOR_25519 := $(UNSATURATED_SOLINAS_FUNCTIONS) carry_scmul121666
 WORD_BY_WORD_MONTGOMERY_FUNCTIONS := mul square add sub opp from_montgomery to_montgomery nonzero selectznz to_bytes from_bytes
+FUNCTIONS_FOR_P224 := $(WORD_BY_WORD_MONTGOMERY_FUNCTIONS) scmul2 scmul3 scmul4 scmul8
 UNSATURATED_SOLINAS := src/ExtractionOCaml/unsaturated_solinas
 WORD_BY_WORD_MONTGOMERY := src/ExtractionOCaml/word_by_word_montgomery
 
@@ -180,7 +181,7 @@ $(eval $(call add_curve_keys,p448_solinas_32,UNSATURATED_SOLINAS,'p448',32,'16' 
 $(foreach bw,64 32,$(eval $(call add_curve_keys,p256_$(bw),WORD_BY_WORD_MONTGOMERY,'p256',$(bw),'2^256 - 2^224 + 2^192 + 2^96 - 1',$(WORD_BY_WORD_MONTGOMERY_FUNCTIONS))))
 $(foreach bw,64 32,$(eval $(call add_curve_keys,secp256k1_$(bw),WORD_BY_WORD_MONTGOMERY,'secp256k1',$(bw),'2^256 - 2^32 - 977',$(WORD_BY_WORD_MONTGOMERY_FUNCTIONS))))
 $(foreach bw,64 32,$(eval $(call add_curve_keys,p384_$(bw),WORD_BY_WORD_MONTGOMERY,'p384',$(bw),'2^384 - 2^128 - 2^96 + 2^32 - 1',$(WORD_BY_WORD_MONTGOMERY_FUNCTIONS))))
-$(foreach bw,64 32,$(eval $(call add_curve_keys,p224_$(bw),WORD_BY_WORD_MONTGOMERY,'p224',$(bw),'2^224 - 2^96 + 1',$(WORD_BY_WORD_MONTGOMERY_FUNCTIONS))))
+$(foreach bw,64 32,$(eval $(call add_curve_keys,p224_$(bw),WORD_BY_WORD_MONTGOMERY,'p224',$(bw),'2^224 - 2^96 + 1',$(FUNCTIONS_FOR_P224))))
 $(foreach bw,64,$(eval $(call add_curve_keys,p434_$(bw),WORD_BY_WORD_MONTGOMERY,'p434',$(bw),'2^216 * 3^137 - 1',$(WORD_BY_WORD_MONTGOMERY_FUNCTIONS)))) # 32 is a bit too heavy
 
 # Files taking 30s or less
